#################################################################
#    QualityLink Ontology and Constraints - v0.4.0
#################################################################

# QualityLink prefix
@prefix ql: <http://data.quality-link.eu/ontology/v1#> .
# RDF basics
@prefix rdf: <http://www.w3.org/1999/02/22-rdf-syntax-ns#> .
@prefix rdfs: <http://www.w3.org/2000/01/rdf-schema#> .
@prefix owl: <http://www.w3.org/2002/07/owl#> .
@prefix skos: <http://www.w3.org/2004/02/skos/core#> .
@prefix sh: <http://www.w3.org/ns/shacl#> .
@prefix xsd: <http://www.w3.org/2001/XMLSchema#> .
# European Learning Model (ELM)
@prefix elm: <http://data.europa.eu/snb/model/elm/> .
@prefix loq: <http://data.europa.eu/snb/model/ap/loq-constraints/> .
# Other used ontologies
@prefix foaf: <http://xmlns.com/foaf/0.1/> .
@prefix adms: <http://www.w3.org/ns/adms#> .
@prefix cc: <http://creativecommons.org/ns#> .
@prefix dcterms: <http://purl.org/dc/terms/> .
@prefix dcat: <http://www.w3.org/ns/dcat#> .
@prefix doap: <http://usefulinc.com/ns/doap#> .
@prefix widoco: <https://w3id.org/widoco/vocab#> .

@base <http://data.quality-link.eu/ontology/v1#> .

<http://data.quality-link.eu/ontology/v1#>
    a owl:Ontology ;
    owl:imports elm: ;
    cc:attributionName "QualityLink project"@en ;
    cc:attributionURL <https://quality-link.eu/> ;
    dcterms:abstract "The QualityLink ontology and application profile build on the European Learning Model (ELM). They defines additional classes and properties to describe things not currently covered in ELM."@en ;
    widoco:introduction "This ontology and application profile were developed as part of the QualityLink Erasmus+ project."@en ;
    dcterms:created "2025-02-13"^^xsd:date ;
    dcterms:license <https://creativecommons.org/licenses/by/4.0/> ;
    dcterms:modified "2025-11-28"^^xsd:date ;
    dcterms:publisher <https://quality-link.eu/> ;
    dcterms:title "QualityLink Ontology and Application Profile"@en ;
    rdfs:label "QualityLink"@en ;
    dcterms:description """The QualityLink ontology extends the European Learning Model (ELM) ontology by additional classes and properties required in the context of the QualityLink project.

The additional classes and properties describe things not currently covered in ELM, including certain quality indicators with relevance for the project.

QualityLink further defines an application profile defined as SHACL constraints, which are based on the ELM Learning Opportunities and Qualifications (LOQ) application profile. The application profile is used by the QualityLink pilot aggregator. The QualityLink profile only adds optional properties to the ELM profile, no required ones.

The profile references the [ELM controlled vocabularies](https://op.europa.eu/en/web/eu-vocabularies/europasstables) published by the EU."""@en ;
    doap:repository <https://github.com/Knowledge-Innovation-Centre/quality-link-specs> ;
    dcat:distribution [
        dcterms:format <https://www.iana.org/assignments/media-types/text/turtle> ;
        dcat:downloadURL <https://specs.quality-link.eu/resources/ontology-shacl.ttl> ;
    ], [
        dcterms:format <https://www.iana.org/assignments/media-types/application/ld+json> ;
        dcat:downloadURL <https://specs.quality-link.eu/resources/ontology-shacl.json> ;
    ], [
        dcterms:format <https://www.iana.org/assignments/media-types/application/rdf+xml> ;
        dcat:downloadURL <https://specs.quality-link.eu/resources/ontology-shacl.rdf> ;
    ], [
        dcterms:format <https://www.iana.org/assignments/media-types/application/n-triples> ;
        dcat:downloadURL <https://specs.quality-link.eu/resources/ontology-shacl.nt> ;
    ] ;
    owl:versionInfo "1.0.0-alpha" .


#################################################################
#    Classes and Shapes
#################################################################

###  http://data.quality-link.eu/ontology/v1#HigherEducationInstitution
ql:HigherEducationInstitution
    a owl:Class, sh:NodeShape ;
    rdfs:subClassOf elm:Organisation ;
    sh:node loq:OrganisationShape ;
    rdfs:label "Higher Education Institution"@en ;
    rdfs:comment "An entity that has full degree awarding powers at higher education level (i.e. EQF levels 5 to 8; QF-EHEA cycle first to third) recognised by at least one national authority."@en ;
    sh:order 30 ;
    sh:property [
        sh:name "identifier"@en ;
        sh:description "ORGREG or SCHAC identifier"@en ;
        sh:or (
            [
                sh:class ql:SchacIdentifier ;
            ]
            [
                sh:class ql:OrgRegIdentifier ;
            ]
        ) ;
        sh:minCount 1;
        sh:path adms:identifier ;
    ], [
        sh:class elm:Organisation ;
        sh:path ql:isMemberOf ;
    ] .

###  http://data.quality-link.eu/ontology/v1#GroupOfHEIs
ql:GroupOfHEIs
    a owl:Class, sh:NodeShape ;
    rdfs:subClassOf elm:Group ;
    sh:node loq:GroupShape ;
    rdfs:label "Group of Higher Education Institutions"@en ;
    rdfs:comment "A group or alliance of higher education institutions"@en ;
    sh:order 33 ;
    sh:property [
        sh:name "has member"@en ;
        sh:class ql:HigherEducationInstitution ;
        sh:minCount 2 ;
        sh:path foaf:member ;
    ] .

###  http://data.quality-link.eu/ontology/v1#EuropeanUniversityAlliance
ql:EuropeanUniversityAlliance
    a owl:Class, sh:NodeShape ;
    rdfs:subClassOf ql:GroupOfHEIs ;
    sh:node ql:GroupOfHEIs ;
    sh:order 34 ;
    rdfs:label "European University Alliance"@en ;
    rdfs:comment "An alliance of higher education institutions that is part of the EU's European Universities programme"@en .

###  http://data.quality-link.eu/ontology/v1#OrgRegIdentifier
ql:OrgRegIdentifier
    a rdfs:Class, sh:NodeShape ;
    rdfs:subClassOf elm:Identifier ;
    sh:node loq:IdentifierShape ;
    rdfs:label "OrgReg ID"@en ;
    rdfs:comment "The identifier assigned to a higher education institution or other organisation in the Register of Public Sector Organisations (OrgReg)"@en ;
    sh:order 31 ;
    sh:property [
        sh:name "scheme ID "@en ;
        sh:description "Identification of the scheme."@en ;
        sh:minCount 1 ;
        sh:maxCount 1 ;
        sh:path <http://data.europa.eu/snb/model/elm/schemeId> ;
        sh:hasValue ql:OrgReg ;
    ], [
        sh:name "identifier"@en ;
        sh:description "The OrgReg identifier of the format XX1111."@en ;
        sh:maxCount 1 ;
        sh:minCount 1 ;
        sh:nodeKind sh:Literal ;
        sh:pattern "^(INT|[A-Z]{2})[0-9]{4}$" ;
        sh:path skos:notation ;
    ] .

###  http://data.quality-link.eu/ontology/v1#SchacIdentifier
ql:SchacIdentifier
    a owl:Class, sh:NodeShape ;
    rdfs:subClassOf elm:Identifier ;
    sh:node loq:IdentifierShape ;
    rdfs:label "SCHAC Code"@en ;
    rdfs:comment "The SCHAC code (schacHomeOrganization) is a domain name used to identify a higher education institution."@en ;
    sh:order 32 ;
    sh:property [
        sh:name "scheme ID "@en ;
        sh:description "Identification of the scheme."@en ;
        sh:minCount 1 ;
        sh:maxCount 1 ;
        sh:path <http://data.europa.eu/snb/model/elm/schemeId> ;
        sh:hasValue ql:Schac ;
    ], [
        sh:name "identifier"@en ;
        sh:description "The SCHAC (schacHomeOrganisation) identifier. Must be a valid DNS domain name."@en ;
        sh:maxCount 1 ;
        sh:minCount 1 ;
        sh:nodeKind sh:Literal ;
        sh:path skos:notation ;
    ] .


###  http://data.quality-link.eu/ontology/v1#LearnerGroupConditions
ql:LearnerGroupConditions
    a owl:Class, sh:NodeShape ;
    rdfs:label "Learner Group Conditions"@en ;
    rdfs:comment "Defines specific conditions for a defined target group of learners to whom a Learning Opportunity is offered, e.g. specific fees or registration portals"@en ;
    sh:order 20 ;
    sh:property [
        sh:minCount 1 ;
        sh:path ql:learnerGroup ;
        sh:class ql:LearnerGroup ;
        sh:order 1 ;
    ], [
        sh:description "Link to a portal where students can register for the learning opportunity (specific for this group of learners)."@en ;
        sh:maxCount 1 ;
        sh:path ql:registrationPortal ;
        sh:datatype xsd:anyURI ;
        sh:order 30 ;
    ], [
        sh:name "fees"@en ;
        sh:description "Information about the pricing of the course, applicable for this specific target group."@en ;
        sh:path elm:priceDetail ;
        sh:class elm:PriceDetail ;
        sh:order 50 ;
    ], [
        sh:description "Number of learners from the specific group that can be enrolled."@en ;
        sh:path ql:enrolmentCapacity ;
        sh:datatype xsd:nonNegativeInteger ;
        sh:order 44 ;
    ], [
        sh:description "Number of learners from the specific group that are currently enrolled."@en ;
        sh:path ql:enrolledLearnerCount ;
        sh:datatype xsd:nonNegativeInteger ;
        sh:order 46 ;
    ], [
        sh:description "Number of learners from the specific group that need to at least enrol for the instance to take place."@en ;
        sh:path ql:enrolmentMinimum ;
        sh:datatype xsd:nonNegativeInteger ;
        sh:order 48 ;
    ], [
        sh:name "admissions procedure"@en ;
        sh:description "Information on how to apply for this specific group of learners."@en ;
        sh:maxCount 1 ;
        sh:path elm:admissionProcedure ;
        sh:class elm:Note ;
        sh:order 40 ;
    ], [
        sh:name "entry requirement"@en ;
        sh:description "Entry requirement or prerequisites that apply to this specific group of learners."@en ;
        sh:maxCount 1 ;
        sh:path elm:entryRequirement ;
        sh:class elm:Note ;
        sh:order 42 ;
    ] .


###  http://data.quality-link.eu/ontology/v1#LearnerGroup
ql:LearnerGroup
    a owl:Class, sh:NodeShape ;
    rdfs:label "Learner Group"@en ;
    rdfs:comment "Defines a target group of learners to whom a Learning Opportunity is offered, e.g. students of a specific alliance or HEI"@en ;
    sh:order 21 ;
    sh:property [
        sh:uniqueLang true ;
        sh:name "title"@en ;
        sh:description "The title of the target group of learners."@en ;
        sh:datatype rdf:langString ;
        sh:path dcterms:title ;
        sh:order 1 ;
    ], [
        sh:uniqueLang true ;
        sh:name "description"@en ;
        sh:description "A free text description of the target group of learners."@en ;
        sh:datatype rdf:langString ;
        sh:path dcterms:description ;
        sh:order 3 ;
    ], [
        sh:name "identifier"@en ;
        sh:description "An identifier for this specific target group of learners."@en ;
        sh:class <http://data.europa.eu/snb/model/elm/Identifier> ;
        sh:path <http://www.w3.org/ns/adms#identifier> ;
        sh:order 10 ;
    ], [
        sh:name "home institutions"@en ;
        sh:description "Defines the group as students from these higher education institution(s)"@en ;
        sh:or (
            [
                sh:class ql:HigherEducationInstitution ;
            ]
            [
                sh:class ql:GroupOfHEIs ;
            ]
        ) ;
        sh:path ql:studentsOf ;
        sh:order 22 ;
    ], [
        sh:description "Defines the group as learners who are not enrolled as students"@en ;
        sh:maxCount 1 ;
        sh:path ql:isOpenToNonEnrolled ;
        sh:datatype xsd:boolean ;
        sh:order 20 ;
    ], [
        sh:description "Defines the group as students following a specific other learning opportunity"@en ;
        sh:path ql:limitLearningOpportunity ;
        sh:or (
            [
                sh:class ql:LearningOpportunitySpecificationReference ;
            ]
            [
                sh:class ql:LearningOpportunityInstanceReference ;
            ]
        ) ;
        sh:order 24 ;
    ], [
        sh:name "specific field"@en ;
        sh:description "Defines the group asstudents from (a) specific field(s) of study; use ISCED-F controlled vocabulary"@en ;
        sh:path elm:limitField ;
        sh:class skos:Concept ;
        sh:order 26 ;
    ], [
        sh:description "Defines the group as students enrolled in another learning opportunity at a specified EQF level or higher; use the EQF controlled vocabulary"@en ;
        sh:path ql:minimumEQFLevel ;
        sh:class skos:Concept ;
        sh:order 28 ;
    ], [
        sh:name "information note"@en ;
        sh:description "Additional information about the defined group of learners"@en ;
        sh:class <http://data.europa.eu/snb/model/elm/Note> ;
        sh:path <http://data.europa.eu/snb/model/elm/additionalNote> ;
        sh:order 29 ;
    ] .


###  http://data.quality-link.eu/ontology/v1#LearningOpportunitySpecification
ql:LearningOpportunitySpecification
    a owl:Class, sh:NodeShape ;
    rdfs:subClassOf elm:LearningAchievementSpecification ;
    rdfs:label "Learning Opportunity Specification"@en ;
    rdfs:comment """The asbtract specification of an opportunity to acquire a given set of learning outcomes, e.g. the general specification of a course, programme or module offered by an education provider.

This class and its shape are based on the ELM *LearningAchievementSpecificationShape* and *QualificationShape*.

Different from the ELM LOQ profile, the shapes are defined as open. Properties that are not used/interpreted by the QualityLink data aggregator have been omitted to simplify the shapes."""@en ;
    sh:order 1 ;
    sh:property [
        sh:name "publisher"@en ;
        sh:description "Publisher, typically the education provider that will offer instances of this learning opportunity; if not provided, the publisher will be inferred to be the institution providing the data source."@en ;
        sh:class ql:HigherEducationInstitution ;
        sh:path dcterms:publisher ;
        sh:order 1 ;
    ], [
        sh:name "identifier"@en ;
        sh:description "Identifier or code, normally assigned by the publisher"@en ;
        sh:minCount 1 ;
        sh:class <http://data.europa.eu/snb/model/elm/Identifier> ;
        sh:path <http://www.w3.org/ns/adms#identifier> ;
        sh:order 10 ;
    ], [
        sh:name "qualification code"@en ;
        sh:description "Identifying code from a qualification-based reference semantic asset, normally assigned by a different entity than the publisher, e.g. a national qualifications authority"@en ;
        sh:class skos:Concept ;
        sh:path <http://data.europa.eu/snb/model/elm/qualificationCode> ;
        sh:order 12 ;
    ], [
        sh:uniqueLang true ;
        sh:name "title"@en ;
        sh:description "Primary name or title; one value per language is permitted"@en ;
        sh:minCount 1 ;
        sh:datatype rdf:langString ;
        sh:path dcterms:title ;
        sh:order 20 ;
    ], [
        sh:name "alternative name"@en ;
        sh:description "Alternative name(s)"@en ;
        sh:datatype rdf:langString ;
        sh:path skos:altLabel ;
        sh:order 22 ;
    ], [
        sh:uniqueLang true ;
        sh:name "description"@en ;
        sh:description "Free text description of the learning opportunity; one value per language is permitted"@en ;
        sh:datatype rdf:langString ;
        sh:path dcterms:description ;
        sh:order 24 ;
    ], [
        sh:name "more information"@en ;
        sh:description "Additional free text note(s)"@en ;
        sh:class <http://data.europa.eu/snb/model/elm/Note> ;
        sh:path <http://data.europa.eu/snb/model/elm/additionalNote> ;
        sh:order 26 ;
    ], [
        sh:name "homepage"@en ;
        sh:description "Web page of the learning opportunity"@en ;
        sh:class <http://data.europa.eu/snb/model/elm/WebResource> ;
        sh:path foaf:homepage ;
        sh:order 28 ;
    ], [
        sh:name "learning outcomes"@en ;
        sh:description "Intended learning outcomes (one by one)"@en ;
        sh:minCount 1 ;
        sh:class <http://data.europa.eu/snb/model/elm/LearningOutcome> ;
        sh:path <http://data.europa.eu/snb/model/elm/learningOutcome> ;
        sh:order 30 ;
    ], [
        sh:name "learning outcome summary"@en ;
        sh:description "Summary of the intended learning outcomes"@en ;
        sh:maxCount 1 ;
        sh:class <http://data.europa.eu/snb/model/elm/Note> ;
        sh:path <http://data.europa.eu/snb/model/elm/learningOutcomeSummary> ;
        sh:order 32 ;
    ], [
        sh:name "language"@en ;
        sh:description "Language(s) in which this learning opportunity is offered; should be provided using the Language Named Authority List"@en ;
        sh:minCount 1 ;
        sh:class skos:Concept ;
        sh:path dcterms:language ;
        sh:order 40 ;
    ], [
        sh:name "thematic area"@en ;
        sh:description "Field according to the ISCED-F 2013 Classification; should be provided using the ISCED-F controlled vocabulary"@en ;
        sh:minCount 1 ;
        sh:class skos:Concept ;
        sh:path <http://data.europa.eu/snb/model/elm/ISCEDFCode> ;
        sh:order 50 ;
    ], [
        sh:name "education subject"@en ;
        sh:description "Field of education from another semantic framework than ISCED-F"@en ;
        sh:class skos:Concept ;
        sh:path <http://data.europa.eu/snb/model/elm/educationSubject> ;
        sh:order 52 ;
    ], [
        sh:name "EQF level"@en ;
        sh:description "Level as specified by the European Qualification Framework (EQF); should be provided using the EQF controlled vocabulary"@en ;
        sh:maxCount 1 ;
        sh:minCount 1 ;
        sh:class skos:Concept ;
        sh:path <http://data.europa.eu/snb/model/elm/EQFLevel> ;
        sh:order 60 ;
    ], [
        sh:name "partial qualification"@en ;
        sh:description "Indicates whether a qualification is a full qualification or part of another qualification"@en ;
        sh:maxCount 1 ;
        sh:datatype xsd:boolean ;
        sh:path <http://data.europa.eu/snb/model/elm/isPartialQualification> ;
        sh:order 62 ;
    ], [
        sh:name "NQF level"@en ;
        sh:description "Level as specified by the relevant national qualification framework(s); should be provided using the Qualifications Framework controlled vocabulary"@en ;
        sh:class skos:Concept ;
        sh:path <http://data.europa.eu/snb/model/elm/NQFLevel> ;
        sh:order 64 ;
    ], [
        sh:name "credit points"@en ;
        sh:description "Credit points allocated; should be using ECTS"@en ;
        sh:class <http://data.europa.eu/snb/model/elm/CreditPoint> ;
        sh:path <http://data.europa.eu/snb/model/elm/creditPoint> ;
        sh:order 70 ;
    ], [
        sh:name "workload"@en ;
        sh:description "Estimation of the time the learner would need to complete all learning activities (e.g. lectures, seminars, projects, practical work, traineeships and individual or self-directed study, including exam preparation) to achieve the learning outcomes"@en ;
        sh:maxCount 1 ;
        sh:datatype xsd:duration ;
        sh:path <http://data.europa.eu/snb/model/elm/volumeOfLearning> ;
        sh:order 72 ;
    ], [
        sh:name "type"@en ;
        sh:description "Category, provided using the Learning opportunity type controlled vocabulary"@en ;
        sh:class skos:Concept ;
        sh:path dcterms:type ;
        sh:order 80 ;
    ], [
        sh:name "category"@en ;
        sh:description "Category, provided as free-text string"@en ;
        sh:datatype rdf:langString ;
        sh:path <http://data.europa.eu/snb/model/elm/category> ;
        sh:order 82 ;
    ], [
        sh:name "target group"@en ;
        sh:description "Specific target group or category of learners for which this learning opportunity is designed; should be provided using the Target group controlled vocabulary"@en ;
        sh:class skos:Concept ;
        sh:path <http://data.europa.eu/snb/model/elm/targetGroup> ;
        sh:order 100 ;
    ], [
        sh:name "entry requirement"@en ;
        sh:description "Entry requirement or prerequisites, described as free text"@en ;
        sh:maxCount 1 ;
        sh:class <http://data.europa.eu/snb/model/elm/Note> ;
        sh:path <http://data.europa.eu/snb/model/elm/entryRequirement> ;
        sh:order 110 ;
    ], [
        sh:path ql:entryRequirementLearningOpportunity ;
        sh:class ql:LearningOpportunitySpecificationReference ;
        sh:order 112 ;
    ], [
        sh:path ql:entryRequirementLearningOutcome ;
        sh:class elm:LearningOutcome ;
        sh:order 114 ;
    ], [
        sh:name "proven by"@en ;
        sh:description "Description of the assessment methods"@en ;
        sh:class <http://data.europa.eu/snb/model/elm/LearningAssessmentSpecification> ;
        sh:path <http://data.europa.eu/snb/model/elm/provenBy> ;
        sh:order 120 ;
    ], [
        sh:path elm:gradingScheme ;
        sh:class elm:GradingScheme ;
        sh:maxCount 1 ;
        sh:name "grading scheme"@en ;
        sh:description "Information on the grading scheme used, optionally incl. grade distribution information"@en ;
        sh:order 130 ;
    ], [
        sh:path ql:passingRate ;
        sh:datatype xsd:nonNegativeInteger ;
        sh:order 132 ;
    ], [
        sh:path ql:isActive ;
        sh:datatype xsd:boolean ;
        sh:order 300 ;
    ], [
        sh:nodeKind sh:Literal ;
        sh:path ql:version ;
        sh:order 310 ;
    ], [
        sh:class ql:LearningOpportunitySpecificationReference ;
        sh:path ql:superseded ;
        sh:order 320 ;
    ], [
        sh:name "is part of"@en ;
        sh:description "Another learning opportunity of which this one is a part, e.g. a course can be part of a programme"@en ;
        sh:class ql:LearningOpportunitySpecificationReference ;
        sh:path <http://data.europa.eu/snb/model/elm/isPartOf> ;
        sh:order 330 ;
    ], [
        sh:name "has part"@en ;
        sh:description "Another learning opportunity that is part of this one, e.g. a programme can consist of several courses"@en ;
        sh:class ql:LearningOpportunitySpecificationReference ;
        sh:path <http://data.europa.eu/snb/model/elm/hasPart> ;
        sh:order 340 ;
    ], [
        sh:name "specialisation of"@en ;
        sh:description "A specification (e.g. a qualification standard) that this learning opportunity implements"@en ;
        sh:class ql:LearningOpportunitySpecificationReference ;
        sh:path <http://data.europa.eu/snb/model/elm/specialisationOf> ;
        sh:order 350 ;
    ], [
        sh:name "instance"@en ;
        sh:description "A concrete instance or offering of this specification"@en ;
        sh:class ql:LearningOpportunityInstance ;
        sh:path elm:learningOpportunity ;
        sh:order 400 ;
    ], [
        sh:name "banner image"@en ;
        sh:description "An image that can be used for display of this learning opportunity"@en ;
        sh:maxCount 1 ;
        sh:class <http://data.europa.eu/snb/model/elm/MediaObject> ;
        sh:path <http://data.europa.eu/snb/model/elm/bannerImage> ;
        sh:order 500 ;
    ], [
        sh:name "last modified"@en ;
        sh:description "Date when the specification was last modified"@en ;
        sh:maxCount 1 ;
        sh:datatype xsd:dateTime ;
        sh:path dcterms:modified ;
        sh:order 999 ;
    ] .

###  http://data.quality-link.eu/ontology/v1#LearningOpportunityInstance
ql:LearningOpportunityInstance
    a owl:Class, sh:NodeShape ;
    rdfs:subClassOf elm:LearningOpportunity ;
    rdfs:label "Learning Opportunity Instance"@en ;
    rdfs:comment "A concrete instance or offering of a learning opportunity, e.g. a course, programme or module as offered in a specific academic year or semester."@en ;
    sh:order 10 ;
    sh:property [
        sh:name "learning opportunity specification"@en ;
        sh:maxCount 1 ;
        sh:minCount 1 ;
        sh:description "Specification of which this is an instance"@en ;
        sh:class ql:LearningOpportunitySpecification ;
        sh:path <http://data.europa.eu/snb/model/elm/learningAchievementSpecification> ;
        sh:order 1 ;
    ], [
        sh:name "provided by"@en ;
        sh:description "The institution(s) providing this instance of the learning opportunity"@en ;
        sh:minCount 1 ;
        sh:class ql:HigherEducationInstitution ;
        sh:path <http://data.europa.eu/snb/model/elm/providedBy> ;
        sh:order 10 ;
    ], [
        sh:name "identifier"@en ;
        sh:description "An identifier of this instance or offering, assigned by the provider"@en ;
        sh:class <http://data.europa.eu/snb/model/elm/Identifier> ;
        sh:path <http://www.w3.org/ns/adms#identifier> ;
        sh:order 20 ;
    ], [
        sh:uniqueLang true ;
        sh:name "title"@en ;
        sh:description "Primary name or title of this instance, if different from the specification; one value per language is permitted"@en ;
        sh:datatype rdf:langString ;
        sh:path dcterms:title ;
        sh:order 30 ;
    ], [
        sh:uniqueLang true ;
        sh:name "description"@en ;
        sh:description "Free text description of this instance/offering; one value per language is permitted"@en ;
        sh:datatype rdf:langString ;
        sh:path dcterms:description ;
        sh:order 32 ;
    ], [
        sh:name "more information"@en ;
        sh:description "Additional free text note(s)"@en ;
        sh:class <http://data.europa.eu/snb/model/elm/Note> ;
        sh:path <http://data.europa.eu/snb/model/elm/additionalNote> ;
        sh:order 34 ;
    ], [
        sh:node <http://data.europa.eu/snb/model/ap/loq-constraints/URLRegexRestriction> ;
        sh:name "homepage"@en ;
        sh:description "Web page of this particular instance/offering"@en ;
        sh:class <http://data.europa.eu/snb/model/elm/WebResource> ;
        sh:path foaf:homepage ;
        sh:order 40 ;
    ], [
        sh:maxCount 1 ;
        sh:datatype xsd:anyURI ;
        sh:path ql:registrationPortal ;
        sh:order 42 ;
    ], [
        sh:node <http://data.europa.eu/snb/model/ap/loq-constraints/URLRegexRestriction> ;
        sh:name "other documents"@en ;
        sh:description "A public web document containing additional documentation about the Learning Opportunity."@en ;
        sh:class <http://data.europa.eu/snb/model/elm/WebResource> ;
        sh:path <http://data.europa.eu/snb/model/elm/supplementaryDocument> ;
        sh:order 44 ;
    ], [
        sh:class ql:LearnerGroupConditions ;
        sh:path ql:learnerGroupConditions ;
        sh:order 50 ;
    ], [
        sh:name "language"@en ;
        sh:description "Language in which this instance is delivered; should be provided using the Language Named Authority List"@en ;
        sh:maxCount 1 ;
        sh:minCount 1 ;
        sh:class skos:Concept ;
        sh:path <http://data.europa.eu/snb/model/elm/defaultLanguage> ;
        sh:order 60 ;
    ], [
        sh:name "mode"@en ;
        sh:description "Mode of learning and assessment, provided using the Modes of learning and assessment controlled vocabulary"@en ;
        sh:class skos:Concept ;
        sh:path <http://data.europa.eu/snb/model/elm/mode> ;
        sh:order 70 ;
    ], [
        sh:name "location"@en ;
        sh:description "Location where this instance/offering is delivered"@en ;
        sh:class dcterms:Location ;
        sh:path <http://data.europa.eu/snb/model/elm/location> ;
        sh:order 80 ;
    ], [
        sh:name "learning schedule"@en ;
        sh:description "The type of schedule in which this instance is delivered; should be provided using the Learning schedule type controlled vocabulary."@en ;
        sh:maxCount 1 ;
        sh:class skos:Concept ;
        sh:path <http://data.europa.eu/snb/model/elm/learningSchedule> ;
        sh:order 90 ;
    ], [
        sh:name "term"@en ;
        sh:description "Period of time in which this instance is offered, e.g. a semester"@en ;
        sh:maxCount 1 ;
        sh:class dcterms:PeriodOfTime ;
        sh:path dcterms:temporal ;
        sh:order 92 ;
    ], [
        sh:name "schedule information"@en ;
        sh:description "Detailed information about the timetable or schedule, may include weekly schedules (e.g. 'Every Monday, 4pm') or the overall schedule (e.g. October: lectures, November: group-work, December: break, January: assessment)"@en ;
        sh:maxCount 1 ;
        sh:class <http://data.europa.eu/snb/model/elm/Note> ;
        sh:path <http://data.europa.eu/snb/model/elm/scheduleInformation> ;
        sh:order 94 ;
    ], [
        sh:name "duration"@en ;
        sh:description "The duration during which this instance will be offered"@en ;
        sh:maxCount 1 ;
        sh:datatype xsd:duration ;
        sh:path <http://data.europa.eu/snb/model/elm/duration> ;
        sh:order 96 ;
    ], [
        sh:name "admissions procedure"@en ;
        sh:description "Information on how to apply for this instance/offering"@en ;
        sh:maxCount 1 ;
        sh:class <http://data.europa.eu/snb/model/elm/Note> ;
        sh:path <http://data.europa.eu/snb/model/elm/admissionProcedure> ;
        sh:order 100 ;
    ], [
        sh:name "application deadline"@en ;
        sh:description "The deadline for applying for this instance/offering"@en ;
        sh:datatype xsd:dateTime ;
        sh:path <http://data.europa.eu/snb/model/elm/applicationDeadline> ;
        sh:order 102 ;
    ], [
        sh:path ql:enrolmentCapacity ;
        sh:datatype xsd:nonNegativeInteger ;
        sh:order 104 ;
    ], [
        sh:path ql:enrolledLearnerCount ;
        sh:datatype xsd:nonNegativeInteger ;
        sh:order 106 ;
    ], [
        sh:path ql:enrolmentMinimum ;
        sh:datatype xsd:nonNegativeInteger ;
        sh:order 108 ;
    ], [
        sh:name "fees"@en ;
        sh:description "Information about the pricing or tuition fees"@en ;
        sh:class <http://data.europa.eu/snb/model/elm/PriceDetail> ;
        sh:path <http://data.europa.eu/snb/model/elm/priceDetail> ;
        sh:order 110 ;
    ], [
        sh:name "grant"@en ;
        sh:description "Information on grant possibilities"@en ;
        sh:class <http://data.europa.eu/snb/model/elm/Grant> ;
        sh:path <http://data.europa.eu/snb/model/elm/grant> ;
        sh:order 112 ;
    ], [
        sh:name "learning activity specification"@en ;
        sh:maxCount 1 ;
        sh:description "Detailed information on the learning activities, including the curricula"@en ;
        sh:class <http://data.europa.eu/snb/model/elm/LearningActivitySpecification> ;
        sh:path <http://data.europa.eu/snb/model/elm/learningActivitySpecification> ;
        sh:order 120 ;
    ], [
        sh:path ql:virtualLearningEnvironment ;
        sh:class skos:Concept ;
        sh:order 122 ;
    ], [
        sh:name "banner image"@en ;
        sh:description "An image that can be used for display of this instance"@en ;
        sh:maxCount 1 ;
        sh:class <http://data.europa.eu/snb/model/elm/MediaObject> ;
        sh:path <http://data.europa.eu/snb/model/elm/bannerImage> ;
        sh:order 200 ;
    ], [
        sh:name "last modification date"@en ;
        sh:description "The date when the learning opportunity was last modified."@en ;
        sh:maxCount 1 ;
        sh:datatype xsd:dateTime ;
        sh:path dcterms:modified ;
        sh:order 999 ;
    ] .


###  http://data.quality-link.eu/ontology/v1#LearningOpportunitySpecificationReference
ql:LearningOpportunitySpecificationReference
    a owl:Class, sh:NodeShape ;
    rdfs:label "Learning Opportunity Specification Reference"@en ;
    rdfs:comment "A reference to another Learning Opportunity specification, identified by a provider and a (local) identifier, without further details."@en ;
    sh:order 2 ;
    sh:property [
        sh:name "provided by"@en ;
        sh:description "Higher Education Institution that offers the LO."@en ;
        sh:class ql:HigherEducationInstitution ;
        sh:minCount 1;
        sh:maxCount 1;
        sh:path elm:providedBy ;
        sh:order 1 ;
    ], [
        sh:name "(local) identifier"@en ;
        sh:description "Identifier of the Learning Opportunity Specification. Must be unique within the scope of the institution identified with providedBy."@en ;
        sh:class elm:Identifier ;
        sh:minCount 1;
        sh:maxCount 1;
        sh:path adms:identifier ;
        sh:order 2 ;
    ] .

###  http://data.quality-link.eu/ontology/v1#LearningOpportunityInstanceReference
ql:LearningOpportunityInstanceReference
    a owl:Class, sh:NodeShape ;
    rdfs:label "Learning Opportunity Instance Reference"@en ;
    rdfs:comment "A reference to another Learning Opportunity Instance, identified by a provider and a (local) identifier, without further details."@en ;
    sh:order 11 ;
    sh:property [
        sh:name "provided by"@en ;
        sh:description "Higher Education Institution that offers the LO."@en ;
        sh:class ql:HigherEducationInstitution ;
        sh:minCount 1;
        sh:maxCount 1;
        sh:path elm:providedBy ;
        sh:order 1 ;
    ], [
        sh:name "(local) identifier"@en ;
        sh:description "Identifier of the Learning Opportunity instance. Must be unique within the scope of the institution identified with providedBy."@en ;
        sh:class elm:Identifier ;
        sh:minCount 1;
        sh:maxCount 1;
        sh:path adms:identifier ;
        sh:order 2 ;
    ] .

###  http://data.quality-link.eu/ontology/v1#GradingSchemeSchape
ql:GradingSchemeSchape
    a sh:NodeShape ;
    sh:targetClass elm:GradingScheme ;
    rdfs:label "Grading Scheme"@en ;
    rdfs:comment "Information on the grading scheme used."@en ;
    sh:order 40 ;
    sh:property [
        sh:name "title"@en ;
        sh:description "The title of the grading scheme. One value per language is permitted."@en ;
        sh:uniqueLang true ;
        sh:datatype rdf:langString ;
        sh:path dcterms:title ;
        sh:order 10 ;
    ], [
        sh:name "identifier"@en ;
        sh:description "An identifier of the grading scheme."@en ;
        sh:class elm:Identifier ;
        sh:path adms:identifier ;
        sh:order 1 ;
    ], [
        sh:name "description"@en ;
        sh:description "A free text description of the grading scheme."@en ;
        sh:uniqueLang true ;
        sh:datatype rdf:langString ;
        sh:path dcterms:description ;
        sh:order 12 ;
    ], [
        sh:name "grade distribution"@en ;
        sh:description "Information on the statistical distribution of grades in the scheme."@en ;
        sh:class elm:ResultDistribution ;
        sh:path elm:resultDistribution ;
        sh:order 20 ;
    ], [
        sh:name "other documents"@en ;
        sh:description "A public web document containing additional documentation about the grading scheme."@en ;
        sh:class elm:WebResource ;
        sh:path elm:supplementaryDocument ;
        sh:order 14 ;
    ] .

###  http://data.quality-link.eu/ontology/v1#GradeDistributionShape
ql:GradeDistributionShape
    a sh:NodeShape ;
    sh:targetClass elm:ResultDistribution ;
    rdfs:label "Grade Distribution "@en ;
    rdfs:comment "It describes a histogram of grades achieved by learners within a specific reference group."@en ;
    sh:order 42 ;
    sh:property [
        sh:class ql:LearnerGroup ;
        sh:path ql:referenceGroup ;
        sh:maxCount 1 ;
        sh:order 10 ;
    ], [
        sh:name "grade"@en ;
        sh:description "One specific grade in the grading scheme with the distribution information."@en ;
        sh:class elm:ResultCategory ;
        sh:path elm:resultCategory ;
        sh:minCount 1 ;
        sh:order 20 ;
    ] .

###  http://data.quality-link.eu/ontology/v1#GradeShape
ql:GradeShape
    a sh:NodeShape ;
    sh:targetClass elm:ResultCategory ;
    rdfs:label "Grade"@en ;
    rdfs:comment "Description of a single grade within a histogram of results."@en ;
    sh:order 44 ;
    sh:property [
        sh:name "label"@en ;
        sh:description "The label of the grade according to the grading scheme it is part of, e.g. 'C', '2+' or '10'."@en ;
        sh:datatype xsd:string ;
        sh:path elm:label ;
        sh:minCount 1 ;
        sh:maxCount 1 ;
        sh:order 10 ;
    ], [
        sh:datatype xsd:positiveInteger ;
        sh:path ql:gradeOrder ;
        sh:minCount 1 ;
        sh:maxCount 1 ;
        sh:order 20 ;
    ], [
        sh:datatype xsd:positiveInteger ;
        sh:path ql:gradePercentage ;
        sh:minCount 1 ;
        sh:maxCount 1 ;
        sh:order 30 ;
    ] .

###  http://data.quality-link.eu/ontology/v1#Kajmak
ql:Kajmak
    a owl:Class ;
    rdfs:subClassOf <http://purl.obolibrary.org/obo/FOODON_00001256> ;
    rdfs:comment "Kaymak is a creamy dairy food similar to clotted cream, made from the milk of water buffalo, cows, sheep, or goats in Central Asia, some Balkan countries, some Caucasus countries, the Levant, Turkic regions, Iran and Iraq."@en ;
    dcterms:source <https://en.wikipedia.org/wiki/Kaymak> ;
    rdfs:label "kajmak"@hbs-Latn, "кајмак"@hbs-Cyrl, "кајмак"@mk, "kajmak"@sl, "kaymak"@en .

#################################################################
#    Object Properties
#################################################################

###  http://data.quality-link.eu/ontology/v1#relatedTo
ql:relatedTo rdf:type owl:ObjectProperty ,
                      owl:AsymmetricProperty ;
             rdfs:comment "A relationship between Learning Opportunities or Organisations (abstract)"@en ;
             rdfs:label "related to"@en .


###  http://data.quality-link.eu/ontology/v1#spunOffFrom
ql:spunOffFrom rdf:type owl:ObjectProperty ;
               rdfs:subPropertyOf ql:relatedTo ;
               rdfs:domain elm:Organisation ;
               rdfs:comment "Organisation spun off from another one (i.e. subject newly created by the event, object existed before and after)"@en ;
               rdfs:label "spun off from"@en .


###  http://data.quality-link.eu/ontology/v1#absorbed
ql:absorbed rdf:type owl:ObjectProperty ;
            rdfs:subPropertyOf ql:relatedTo ;
            rdfs:domain elm:Organisation ;
            rdfs:comment "Organisation absorbed another one (i.e. subject existed before and after the event, object ceased to exist)"@en ;
            rdfs:label "absorbed"@en .


###  http://data.quality-link.eu/ontology/v1#succeeded
ql:succeeded rdf:type owl:ObjectProperty ;
             rdfs:subPropertyOf ql:relatedTo ;
             rdfs:domain elm:Organisation ;
             rdfs:comment "Organisation succeeded/replaced another one (i.e. subject was newly created by the event, object ceased to exist)"@en ;
             rdfs:label "succeeded"@en .


###  http://data.quality-link.eu/ontology/v1#superseded
ql:superseded rdf:type owl:ObjectProperty ;
    rdfs:subPropertyOf ql:relatedTo ;
    rdfs:domain ql:LearningOpportunitySpecification ;
    rdfs:comment "Learning Opportunity specification superseded another one, which is no longer (or temporarily not) offered."@en ;
    rdfs:label "superseded"@en .


###  http://data.quality-link.eu/ontology/v1#learnerGroupConditions
ql:learnerGroupConditions rdf:type owl:ObjectProperty ;
               rdfs:domain ql:LearningOpportunityInstance ;
               rdfs:range ql:LearnerGroupConditions ;
               rdfs:comment "Indicates specific conditions that apply to a certain target group of learners" ;
               rdfs:label "specific conditions for learner group"@en .


###  http://data.quality-link.eu/ontology/v1#learnerGroup
ql:learnerGroup rdf:type owl:ObjectProperty ;
               rdfs:domain ql:LearningOpportunityInstance ;
               rdfs:range ql:LearnerGroup ;
               rdfs:comment "Definition of the specific group of learners to whom these conditions apply" ;
               rdfs:label "learner group"@en .


###  http://data.quality-link.eu/ontology/v1#studentsOf
ql:studentsOf rdf:type owl:ObjectProperty ;
              rdfs:domain ql:LearnerGroup ;
              rdfs:comment "Defines that the target group of learners includes the students of an education institution, or an alliance thereof"@en ;
              rdfs:label "includes students of"@en .


###  http://data.quality-link.eu/ontology/v1#limitLearningOpportunity
ql:limitLearningOpportunity rdf:type owl:ObjectProperty ;
    rdfs:domain ql:LearnerGroup ;
    rdfs:comment "Defines that the learning opportunity is offered to students enrolled in a specified other learning opportunity."@en ;
    rdfs:label "specific learning opportunity"@en .


###  http://data.quality-link.eu/ontology/v1#minimumEQFLevel
ql:minimumEQFLevel rdf:type owl:ObjectProperty ;
    rdfs:domain ql:LearnerGroup ;
    rdfs:comment "Defines that the learning opportunity is offered to students enrolled in another learning opportunity at a specified EQF level or higher. If provided, the value must come from the EU controlled vocabulary http://publications.europa.eu/resource/dataset/european-qualification-framework"@en ;
    rdfs:label "minimum EQF Level"@en .


###  http://data.quality-link.eu/ontology/v1#entryRequirementLearningOpportunity
ql:entryRequirementLearningOpportunity rdf:type owl:ObjectProperty ;
    rdfs:range ql:LearningOpportunitySpecificationReference ;
    rdfs:comment "Specific entry requirement or prerequisite to have completed another learning opportunity."@en ;
    rdfs:label "required learning opportunity for entry"@en .


###  http://data.quality-link.eu/ontology/v1#entryRequirementLearningOutcome
ql:entryRequirementLearningOutcome rdf:type owl:ObjectProperty ;
    rdfs:range elm:LearningOutcome ;
    rdfs:comment "Specific entry requirement or prerequisite to have achieved a particular learning outcome."@en ;
    rdfs:label "required learning outcome for entry"@en .


###  http://data.quality-link.eu/ontology/v1#referenceGroup
ql:referenceGroup
    a owl:ObjectProperty ;
    rdfs:domain elm:ResultDistribution ;
    rdfs:range ql:LearnerGroup ;
    rdfs:label "reference group"@en ;
    rdfs:comment "The group of learners for which the histogram of results was established."@en .


###  http://data.quality-link.eu/ontology/v1#virtualLearningEnvironment
ql:virtualLearningEnvironment
    a owl:ObjectProperty ;
    rdfs:domain ql:LearningOpportunityInstance ;
    rdfs:label "virtual learning environment"@en ;
    rdfs:comment "Specifies (a) virtual learning environment(s) used in the delivery of this learning opportunity."@en .


###  http://data.quality-link.eu/ontology/v1#isMemberOf
ql:isMemberOf
    a owl:ObjectProperty ;
    rdfs:label "is member of"@en ;
    rdfs:comment "Specifies that an organisation is member of an association, e.g. an institution member of EUA or EURASHE."@en .


#################################################################
#    Data properties
#################################################################

###  http://data.quality-link.eu/ontology/v1#registrationPortal
ql:registrationPortal rdf:type owl:DatatypeProperty ;
                      rdfs:range xsd:anyURI ;
                      rdfs:comment "A web page at which one can register or enrol for a Learning Opportunity." ;
                      rdfs:label "registration portal"@en .


###  http://data.quality-link.eu/ontology/v1#version
ql:version rdf:type owl:DatatypeProperty ;
    rdfs:range xsd:string ;
    rdfs:comment "A number or other identifier that indicates the version of the Learning Opportunity specifcation." ;
    rdfs:label "version"@en .


###  http://data.quality-link.eu/ontology/v1#isActive
ql:isActive a owl:DatatypeProperty ;
    rdfs:range xsd:boolean ;
    rdfs:comment "Learning Opportunity Specification is active, i.e. instances are currently offered or the education provider expects that instances will still be offered in the future." ;
    rdfs:label "is active"@en .


###  http://data.quality-link.eu/ontology/v1#isOpenToNonEnrolled
ql:isOpenToNonEnrolled a owl:DatatypeProperty ;
    rdfs:range xsd:boolean ;
    rdfs:comment "Indicates that a learning opportunity is alos open to learners not currently enrolled as regular students." ;
    rdfs:label "open to non-enrolled learners"@en .


###  http://data.quality-link.eu/ontology/v1#enrolmentCapacity
ql:enrolmentCapacity a owl:DatatypeProperty ;
    rdfs:range xsd:nonNegativeInteger ;
    rdfs:comment "The number of learners that can register for a Learning Opportunity Instance." ;
    rdfs:label "enrolment capacity"@en .


###  http://data.quality-link.eu/ontology/v1#enrolledLearnerCount
ql:enrolledLearnerCount a owl:DatatypeProperty ;
    rdfs:range xsd:nonNegativeInteger ;
    rdfs:comment "The number of learners that are currently enrolled for the Learning Opportunity Instance." ;
    rdfs:label "enrolled learner count"@en .


###  http://data.quality-link.eu/ontology/v1#enrolmentMinimum
ql:enrolmentMinimum a owl:DatatypeProperty ;
    rdfs:range xsd:nonNegativeInteger ;
    rdfs:comment "The number of learners that at least need to enrole for a Learning Opportunity Instance to take place." ;
    rdfs:label "minimum enrolment"@en .


###  http://data.quality-link.eu/ontology/v1#passingRate
ql:passingRate a owl:DatatypeProperty ;
    rdfs:range xsd:positiveInteger ;
    rdfs:label "passing rate"@en ;
    rdfs:comment "The percentage of learners who pass on average."@en .

###  http://data.quality-link.eu/ontology/v1#gradeOrder
ql:gradeOrder a owl:DatatypeProperty ;
    rdfs:range xsd:positiveInteger ;
    rdfs:label "order"@en ;
    rdfs:comment "A number specifying the order of the grade within the grading scheme, the highest number indicating the best grade."@en .

###  http://data.quality-link.eu/ontology/v1#gradePercentage
ql:gradePercentage a owl:DatatypeProperty ;
    rdfs:range xsd:positiveInteger ;
    rdfs:label "percentage"@en ;
    rdfs:comment "The percentage of learners earning this grade."@en .


#################################################################
#    Individuals
#################################################################

###  http://data.quality-link.eu/ontology/v1#OrgReg
ql:OrgReg rdf:type skos:ConceptScheme ;
          rdfs:comment "The identifier scheme defined by the Register of Public Sector Organisations (OrgReg)"@en ;
          rdfs:label "OrgReg (identifier scheme)"@en .


###  http://data.quality-link.eu/ontology/v1#SchacIdentifier
ql:Schac rdf:type skos:ConceptScheme ;
         rdfs:comment "The identifier scheme for higher education institutions defined by the Schema for Academia (SCHAC)."@en ;
         rdfs:label "SCHAC (identifier scheme)"@en .

